\documentclass[11pt,a4paper]{article}
\usepackage[utf8x]{inputenc}
\usepackage{isolatin1}
\usepackage{ctable}
\usepackage[french]{babel}

%\usepackage[T1]{inputenc}
%\usepackage{float}
%\usepackage{vmargin}
\usepackage{epsfig}
\usepackage{graphicx}
\usepackage{graphics}

\setlength{\parindent}{10pt}
\setlength{\parskip}{10pt}
%\renewcommand{\baselinestretch}{2.0}
%\renewcommand\baselinestretch{1.5}
\newcommand\numero{{n$^{\rm o}\,\,$}}
\input{macros}
\input{nondim}

\begin{document}
\titlepage
\mbox{}
Basic equations
\be
f(u) + s(u) = 0  \hb{and} \nabla \cdot u = 0. 
\nd
where in the Navier-Stokes case
\be
f(u) = \Delta u + g
\nd
and
\be
s(u) = - \nabla p 
\nd
where the pressure is whatever is necessary for incompressibility.
One step of Gauss-Seidel
for the Laplacian operator. 
\be
u^{n,*,k} = M(u^{n,k},g - \nabla p^{k-1}) 
\nd
where for any function $h$
\be
M(v,h) = v \hb{if}  \Delta v + h = 0.
\nd
The next iteration is defined by 
\be
u^{n,k+1} = u^{n,*,k} + \nabla \pi^{k} \hb{and} \nabla \cdot u^{n,k+1} = 0  
\nd
and
\be 
p^k = p^{k-1} + \pi^k.
\nd
At convergence
\be
u^{n,k+1} = u^{n,k}
\nd
and
\be
\pi^k = 0.
\nd
Then
\be
u^{n,k+1}  = M(u^{n,k},g - \nabla p^{k-1}) .
\nd
Let $v = u^{n,k}$ then
\be
v = M(v,g - \nabla p)
\nd
and thus
\be
\Delta v + g - \nabla p = 0 ,
\nd
achieving
\be
f(v) + s(v)  = 0 \hb{and} \nabla \cdot v = 0. 
\nd
\newpage

 
Since
\be
\nabla \cdot f(u) - \Delta p = 0
\nd
then
\be
p = \Delta^{-1} ( \nabla \cdot f(u) ) ,
\nd
(boundary conditions on $p$ are not specified at this point although
I believe that $n \cdot \nabla p = 0$ should work.)
Then if
\be
h(w) = - \nabla \Delta^{-1} ( \nabla \cdot w ) 
\nd
then
\be
s(u) = h[f(u)]
\nd 
with bc on solids. If we solve using a time evolution
\be
\dert u = f(u) + s(u) = 0  \hb{and} \nabla \cdot u = 0. 
\nd
then an explici method is
\be
u^* = u^n + \tau f(u^n)
\nd
and
\be
u^{n+1} = u^* + h(u^*) .
\nd
Implicit:
\be
u^* = u^n + \tau f(u^*)
\nd
and
\be
u^{n+1} = u^* + h(u^*).
\nd
If explicit and $u^{n+1} = u^n = v$ then
\be
v = v + \tau f(v) + \tau h[f(v)] 
\nd
and thus we solve the problem
\be
L(v) = f(v) + h[f(v)] = 0 \hb{and} \nabla \cdot v = 0 
\nd
If implicit and  $u^{n+1} = u^n = v$ then
\be
v = v + \tau f(u^*) + h(u^*) 
\nd
and
so we solve a different problem
\be
h(u^*) + f(u^*) =0 \hb{and} \nabla \cdot v = 0 
\nd
with $v$ related to $u^*$ as above. 

\newpage
\begin{center}
\vskip 1cm
{\Large \bf Note on viscous terms
}\\\vskip 1cm
St√©phane Zaleski\\
\vskip 0.5cm
{\small  \it
D'ALEMBERT\\
} 
\vskip 0.5 cm 
{\it email: zaleski@dalembert.upmc.fr}
\vskip 0.5 cm
\today
\end{center}

\newpage
The viscous term is
\be
\F_v =\nabla \cdot \{ \mu [\nabla\U  + (\nabla\U)^T] \}
= \nabla \mu \cdot [\nabla\U  + (\nabla\U)^T]  + \mu \Delta\U
\nd
The term computed in {\sf MomentumDiffusion} is 
\be
\delta u = \frac 1 {\delta y}  \left( \mu_{i+1/2,j+1/2} \left.\frac {\delta v }{\delta y}\right\vert_{i+1/2,j+1/2} - \mu_{i+1/2,j-1/2} \left.\frac {\delta v }{\delta y}\right\vert_{i+1/2,j-1/2}\right)
\nd
using
$ac - bd =1/2[ (a-b)(c+d) + (a+b)(c-d) ] =1/2[ ac - bd + ad - bc + ac - bd - ad + bc]$

\begin{eqnarray}
\delta u & = & \frac 1 {2 \delta y} \left[  \left( \mu_{i+1/2,j+1/2}  + \mu_{i+1/2,j-1/2}
\right) \left( \left.\frac {\delta v }{\delta y}\right\vert_{i+1/2,j+1/2} - \left.\frac {\delta v }{\delta y}\right\vert_{i+1/2,j-1/2}\right)\right.\nonumber \\
& + &  \left.\left( \mu_{i+1/2,j+1/2}  - \mu_{i+1/2,j-1/2} \right) 
\left( \left.\frac {\delta v }{\delta y}\right\vert_{i+1/2,j+1/2} + \left.\frac {\delta v }{\delta y}\right\vert_{i+1/2,j-1/2}\right)\right]
\end{eqnarray}

\end{document}
